make sure promise type is abstract

iocy/FancyTraces2.fst
@@ -5,88 +5,29 @@ open FStar.Ghost
 
 module M = FStar.FiniteMap.Base
 
-type promise_id = erased nat
+type promise_id = nat
 
 noeq
 type promise (e:Type u#a) (a:Type u#b) : Type u#(max a b) =
 | Promise : id:promise_id -> r:erased a -> promise e a
 (** CA: having the local trace on the promise, pushes the promise type to universe 1, preventing HO promises **)
 
-noeq
-type event (e: Type0) : Type u#1 =
-| Ev : e -> event e
-| EAsync : #b:Type0 -> pr:promise e b -> lt:atrace e -> event e
-| EAwait : #b:Type0 -> pr:promise e b -> event e
-and atrace e : Type u#1 = list (event e)
+let suffix_of l h = admit ()
+let lemma_suffix_of_reflexive l = admit ()
 
-type trace e = list e
-
-assume val suffix_of : atrace 'e -> atrace 'e -> Type0
-assume val lemma_suffix_of_reflexive : l:atrace 'e -> Lemma (suffix_of l l)
-
-type parallel_traces e = (* promise_id -> atrace *)
-  M.map nat (atrace e)
+type parallel_traces e : Type u#1 = (* promise_id -> atrace *)
+  M.map promise_id (atrace e)
   (* CA: this nat should be promise_id, but is not an eqtype? *)
   // M.map int (a:Type0 & pr:promise e a & tr:atrace e)
   (* CA: why do I have the promise here? *)
 
 let mem_id (id:promise_id) (pts:parallel_traces 'e) = reveal id `M.mem` pts
-let sel_id (id:promise_id) (pts:(parallel_traces 'e){id `mem_id` pts}) : GTot (atrace 'e) =
-  M.lookup (reveal id) pts
+let sel_id (id:promise_id) (pts:(parallel_traces 'e){id `mem_id` pts}) : (atrace 'e) =
+  M.lookup id pts
   // Mkdtuple3?._3 (M.lookup id pts)
 
 let mem (pr:promise 'e 'a) (pts:parallel_traces 'e) = pr.id `mem_id` pts
-let sel (pr:promise 'e 'a) (pts:(parallel_traces 'e){pr `mem` pts}) : GTot (atrace 'e) =
+let sel (pr:promise 'e 'a) (pts:(parallel_traces 'e){pr `mem` pts}) :  atrace 'e =
   sel_id pr.id pts
-
-let insert (pr:promise 'e 'a) (lt:atrace 'e) (pts:parallel_traces 'e) : GTot (parallel_traces 'e) =
-  M.insert (reveal pr.id) lt pts
-
-let ord #e (pts pts':parallel_traces e) =
-  (forall x. x `mem_id` pts ==> x `mem_id` pts') /\
-  (forall x. x `mem_id` pts ==> (sel_id x pts' `suffix_of` sel_id x pts))
-
-assume val size : atrace 'e -> nat
-
-let rec closed_atrace (m:parallel_traces 'e) (tr:atrace 'e) : GTot Type0 (decreases (size tr)) =
-  match tr with
-  | [] -> True
-  | Ev _ :: tl ->
-    assume (size tl < size tr);
-    closed_atrace m tl
-  | EAwait #_ #b pr :: tl ->
-    assume (size tl < size tr);
-    pr `mem` m /\ closed_atrace m tl
-  | EAsync pr lt :: tl ->
-    assume (size lt < size tr);
-    assume (size (lt@tl) < size tr);
-    closed_atrace m lt /\
-    closed_atrace (insert pr lt m) (lt@tl)
-    (** this is a bit awkard because it exposes the promise to the asynchronus computation **)
-    (** this variant does not consider HO promises:
-        closed_atrace m lt /\ closed_atrace (map_insert pr m lt) tl **)
-
-val interleave_map
-  (pts: parallel_traces 'e)
-  (#_: squash (forall id. id `mem_id` pts ==> closed_atrace pts (sel_id id pts)))
-  : list (trace 'e)
-
-let w_pre e = h:atrace e -> map:parallel_traces e{
-  closed_atrace map h
-  // /\ (forall pr. pr `map_mem` map ==> (map_sel pr map) `suffix_of` pr.lt)
-  // we cannot have this refinement since we don't store the trace on the promise anymore
-} -> Type0
-
-let w_post e a h pts =
-  a -> lt:atrace e -> pts':parallel_traces e{
-      pts `ord` pts' /\
-      closed_atrace pts' (h @ lt)
-  } -> Type0
-
-let w e a = h:atrace e -> pts:parallel_traces e{closed_atrace pts h} -> w_post e a h pts -> Type0
-
-let encode_pre_post_in_w #e #a
-  (pre:w_pre e)
-  (post:(h:atrace e -> pts:parallel_traces e -> w_post e a h pts))
-  : w e a
-  = (fun h pts p -> pre h pts /\ (forall r' lt' pts'. post h pts r' lt' pts' ==> p r' lt' pts'))
+let insert (pr:promise 'e 'a) (lt:atrace 'e) (pts:parallel_traces 'e) : parallel_traces 'e =
+  M.insert pr.id lt pts
